src/RawRenaming.v
@@ -1,0 +1,59 @@
+Require Import Label PeanoNat Psatz Ring Compare_dec StrictProp.
+Require Import Var VarEquations.
+
+Inductive raw_renaming :=
+  | raw_renaming_id : raw_renaming
+  | raw_renaming_extend :
+      var -> raw_renaming -> var -> raw_renaming.
+
+Fixpoint apply_raw_renaming_var r : var_op 0 0 :=
+  match r with
+  | raw_renaming_id => var_op_id
+  | raw_renaming_extend vl r vr =>
+    pop_var vl @ lift_var_op (apply_raw_renaming_var r) @ push_var vr
+  end.
+
+Set Primitive Projections.
+Record renaming_rhs :=
+  mk_renaming_rhs {
+      rhs_raw_renaming : raw_renaming;
+      rhs_push : var
+    }.
+Add Printing Constructor renaming_rhs.
+Unset Primitive Projections.
+
+Definition renaming_rhs_extend vl r vr :=
+  mk_renaming_rhs
+    (raw_renaming_extend vl
+        (rhs_raw_renaming r)
+        (unshift_var (rhs_push r) vr))
+    (shift_var vr (rhs_push r)).
+
+Fixpoint transpose_push_raw_renaming v r {struct r} :=
+  match r with
+  | raw_renaming_id => mk_renaming_rhs raw_renaming_id v
+  | raw_renaming_extend vl r vr =>
+    if var_eqb v vl then mk_renaming_rhs r vr
+    else renaming_rhs_extend
+           (unshift_var v vl)
+           (transpose_push_raw_renaming (unshift_var vl v) r)
+           vr
+  end.
+
+Fixpoint compose_raw_renaming r1 r2 :=
+  match r1 with
+  | raw_renaming_id => r2
+  | raw_renaming_extend vl r1 vr =>
+    let rhs := transpose_push_raw_renaming vr r2 in
+    raw_renaming_extend
+      vl
+      (compose_raw_renaming r1 (rhs_raw_renaming rhs))
+      (rhs_push rhs)
+  end.
+
+Fixpoint inverse_raw_renaming r :=
+  match r with
+  | raw_renaming_id => r
+  | raw_renaming_extend vl r vr =>
+      raw_renaming_extend vr (inverse_raw_renaming r) vl
+  end.
