src/RawRenamingEquations.v
@@ -1,0 +1,303 @@
+Require Import Label PeanoNat Psatz Ring Compare_dec StrictProp.
+Require Import Var VarEquations RawRenaming.
+
+(* Properties of raw renaming composition *)
+
+Definition apply_renaming_rhs_var r : var_op 0 1 :=
+  lift_var_op (apply_raw_renaming_var (rhs_raw_renaming r))
+  @ push_var (rhs_push r).
+Arguments apply_renaming_rhs_var r /.
+
+(* TODO: move to var equations *)
+Lemma lift_var_op_compose'
+      {L N M O} (op1 : var_op N M) (op2 : var_op L N)
+      (op3 : var_op O (S L)) :
+  lift_var_op (op1 @ op2) @ op3
+  =v= lift_var_op op1 @ (lift_var_op op2 @ op3).
+Proof.
+  rewrite var_op_associative.
+  rewrite lift_var_op_compose.
+  rewrite <- var_op_associative.
+  easy.
+Qed.
+
+(* TODO: move to var equations *)
+Ltac case_vars_eq v1 v2 :=
+  let Hneql := fresh "Hneql" in
+  change (var_eqb v1 v2)
+    with (if var_dec v1 v2 then true else false);
+  destruct (var_dec v1 v2) as [<-|Hneql]; cbn.
+
+Lemma apply_transpose_push_raw_renaming v r :
+  push_var v
+  @ apply_raw_renaming_var r
+  =v=
+  apply_renaming_rhs_var (transpose_push_raw_renaming v r).
+Proof.
+  generalize dependent v.
+  induction r as [|vl r IHr vr]; intros v; cbn.
+  - simplify_var_ops; easy.
+  - case_vars_eq v vl.
+    + rewrite push_pop_identity'; easy.
+    + rewrite transpose_push_pop' by easy.
+      simplify_var_ops.
+      rewrite <- lift_var_op_compose'.
+      rewrite IHr; cbn; simplify_var_ops.
+      rewrite transpose_swap_lifted'.
+      rewrite transpose_pushes.
+      rewrite swap_swap_identity'.
+      easy.
+Qed.
+
+Lemma apply_compose_raw_renaming r1 r2 :
+  apply_raw_renaming_var (compose_raw_renaming r1 r2)
+  =v= apply_raw_renaming_var r1 @ apply_raw_renaming_var r2.
+Proof.
+  generalize dependent r2.
+  induction r1 as [|vl r1 IHr1 vr]; intros r2; cbn; try easy.
+  rewrite IHr1; simplify_var_ops.
+  rewrite apply_transpose_push_raw_renaming.
+  easy.
+Qed.
+
+Lemma raw_renaming_left_identity r :
+  compose_raw_renaming raw_renaming_id r = r.
+Proof. easy. Qed.
+
+Lemma raw_renaming_right_identity r :
+  compose_raw_renaming r raw_renaming_id = r.
+Proof.
+  induction r as [|vl r IHr vr]; cbn; try easy.
+  rewrite IHr; easy.
+Qed.
+
+Fixpoint transpose_push_raw_renaming_push v r {struct r} :=
+  match r with
+  | raw_renaming_id => v
+  | raw_renaming_extend vl r vr =>
+    if var_eqb v vl then vr
+    else shift_var vr
+           (transpose_push_raw_renaming_push
+              (unshift_var vl v) r)
+  end.
+
+Lemma rhs_push_transpose_push_raw_renaming v r :
+  rhs_push (transpose_push_raw_renaming v r)
+  = transpose_push_raw_renaming_push v r.
+Proof.
+  generalize dependent v.
+  induction r as [|vl r IHr vr]; intros v; cbn; try easy.
+  case_vars_eq v vl; try easy.
+  rewrite IHr; easy.
+Qed.
+
+Fixpoint transpose_push_raw_renaming_raw_renaming
+         v r {struct r} :=
+  match r with
+  | raw_renaming_id => raw_renaming_id
+  | raw_renaming_extend vl r vr =>
+    if var_eqb v vl then r
+    else
+      raw_renaming_extend
+        (unshift_var v vl)
+        (transpose_push_raw_renaming_raw_renaming
+           (unshift_var vl v) r)
+        (unshift_var
+           (transpose_push_raw_renaming_push
+              (unshift_var vl v) r)
+           vr)
+
+  end.
+
+Lemma rhs_raw_renaming_transpose_push_raw_renaming v r :
+  rhs_raw_renaming (transpose_push_raw_renaming v r)
+  = transpose_push_raw_renaming_raw_renaming v r.
+Proof.
+  generalize dependent v.
+  induction r as [|vl r IHr vr]; intros v; cbn; try easy.
+  case_vars_eq v vl; try easy.
+  rewrite rhs_push_transpose_push_raw_renaming, IHr; easy.
+Qed.
+
+Lemma renaming_rhs_eta r :
+  r = mk_renaming_rhs (rhs_raw_renaming r) (rhs_push r).
+Proof. easy. Qed.
+
+Lemma transpose_push_raw_renaming_eta vo r :
+  transpose_push_raw_renaming vo r
+  = mk_renaming_rhs
+      (transpose_push_raw_renaming_raw_renaming vo r)
+      (transpose_push_raw_renaming_push vo r).
+Proof.
+  rewrite renaming_rhs_eta
+    with (r := transpose_push_raw_renaming vo r).
+  rewrite rhs_raw_renaming_transpose_push_raw_renaming.
+  rewrite rhs_push_transpose_push_raw_renaming.
+  easy.
+Qed.
+
+Lemma transpose_push_raw_renaming_reverse_right v1 v2 r :
+  shift_var (transpose_push_raw_renaming_push v1 r)
+    (transpose_push_raw_renaming_push v2
+       (transpose_push_raw_renaming_raw_renaming v1 r)) =
+  transpose_push_raw_renaming_push (shift_var v1 v2) r.
+Proof.
+  generalize dependent v1.
+  generalize dependent v2.
+  induction r as [|vl r IHr vr]; intros v2 v1; cbn; try easy.
+  case_vars_eq v1 vl.
+  - rewrite transpose_op_reducing_push_pop.
+
+  case_var_zero vo1.
+  - rewrite transpose_push_reducing_push_pop; easy.
+  - rewrite transpose_push_normalized_pushes_cons_push; cbn.
+    case_var_zero vo2.
+    + apply transpose_pushes_squared_right.
+    + rewrite transpose_pushes_reverse_right.
+      rewrite IHr.
+      rewrite transpose_push_push_pop_zero_reverse_right
+        by easy.
+      easy.
+Qed.
+
+Lemma transpose_push_raw_closing_reverse_middle vo1 vo2 r :
+  unshift_var_opt
+    (transpose_push_raw_closing_push
+       vo1 (transpose_push_raw_closing_raw_closing vo2 r))
+    (transpose_push_raw_closing_push vo2 r)
+  = transpose_push_raw_closing_push
+      (unshift_var_opt vo1 vo2)
+      (transpose_push_raw_closing_raw_closing
+         (shift_var_opt vo2 vo1) r).
+Proof.
+  generalize dependent vo1.
+  generalize dependent vo2.
+  induction r as [|vo3 r]; intros vo2 vo1; cbn; try easy.
+  case_var_zero vo2.
+  - rewrite transpose_push_normalized_pushes_cons_push; cbn.
+    rewrite transpose_push_push_zero_left; cbn.
+    rewrite transpose_push_reducing_push_pop; easy.
+  - rewrite transpose_push_normalized_pushes_cons_push; cbn.
+    case_var_zero vo1.
+    + rewrite transpose_pushes_squared_left.
+      destruct vo2; easy.
+    + rewrite transpose_push_normalized_pushes_cons_push;
+        cbn; reduce_var_zero.
+      rewrite transpose_pushes_reverse_middle.
+      rewrite IHr.
+      rewrite transpose_push_push_pop_zero_reverse_middle.
+      rewrite transpose_push_raw_closing_reverse_right.
+      rewrite transpose_push_push_pop_zero_reverse_right
+        by easy.
+      easy.
+Qed.
+
+Lemma transpose_push_raw_closing_reverse_left vo1 vo2 r :
+  transpose_push_raw_closing_raw_closing vo1
+    (transpose_push_raw_closing_raw_closing vo2 r)
+  = transpose_push_raw_closing_raw_closing
+      (unshift_var_opt vo1 vo2)
+      (transpose_push_raw_closing_raw_closing
+         (shift_var_opt vo2 vo1) r).
+Proof.
+  generalize dependent vo1.
+  generalize dependent vo2.
+  induction r as [|vo3 r]; intros vo2 vo1; cbn; try easy.
+  case_var_zero vo2.
+  - rewrite
+      transpose_push_normalized_pushes_cons_raw_closing; cbn.
+    rewrite transpose_push_push_zero_left; cbn.
+    rewrite transpose_push_reducing_push_pop; easy.
+  - rewrite
+      transpose_push_normalized_pushes_cons_raw_closing; cbn.
+    case_var_zero vo1.
+    + destruct vo2; easy.
+    + rewrite
+        transpose_push_normalized_pushes_cons_raw_closing;
+        cbn; reduce_var_zero.
+      rewrite <- transpose_pushes_reverse_left.
+      rewrite transpose_push_raw_closing_reverse_right.
+      rewrite transpose_push_raw_closing_reverse_middle.
+      rewrite IHr.
+      rewrite transpose_push_push_pop_zero_reverse_middle.
+      rewrite transpose_push_push_pop_zero_reverse_right
+        by easy.
+      easy.
+Qed.
+
+Lemma transpose_push_compose_raw_closing_push r1 r2 vo :
+  transpose_push_raw_closing_push
+    vo (compose_raw_closing r1 r2)
+  = transpose_push_raw_closing_push
+      (transpose_push_raw_closing_push vo r1) r2.
+Proof.
+  generalize dependent vo.
+  generalize dependent r2.
+  induction r1 as [|vo' r1]; intros r2 vo; cbn; try easy.
+  rewrite rhs_push_transpose_push_raw_closing,
+    rhs_raw_closing_transpose_push_raw_closing.
+  rewrite transpose_push_normalized_pushes_cons_push; cbn.
+  case_var_zero vo; try easy.
+  rewrite IHr1.
+  apply transpose_push_raw_closing_reverse_right.
+Qed.
+
+Lemma transpose_push_compose_raw_closing_raw_closing r1 r2 vo :
+  normalized_pushes r2 ->
+  transpose_push_raw_closing_raw_closing
+    vo (compose_raw_closing r1 r2)
+  = compose_raw_closing
+      (transpose_push_raw_closing_raw_closing vo r1)
+      (transpose_push_raw_closing_raw_closing
+         (transpose_push_raw_closing_push vo r1) r2).
+Proof.
+  generalize dependent vo.
+  generalize dependent r2.
+  induction r1 as [|vo' r1]; intros r2 vo Hnorm; cbn; try easy.
+  rewrite rhs_push_transpose_push_raw_closing,
+    rhs_raw_closing_transpose_push_raw_closing.
+  rewrite
+    transpose_push_normalized_pushes_cons_raw_closing; cbn.
+  case_var_zero vo; try easy.
+  rewrite IHr1;
+    try (apply transpose_push_raw_closing_raw_closing_normalized;
+         easy).
+  rewrite transpose_push_raw_closing_reverse_left.
+  rewrite transpose_push_compose_raw_closing_push.
+  rewrite transpose_push_raw_closing_reverse_middle.
+  rewrite compose_normalized_pushes_cons;
+    try (apply transpose_push_raw_closing_raw_closing_normalized;
+         easy); cbn.
+  rewrite rhs_push_transpose_push_raw_closing,
+    rhs_raw_closing_transpose_push_raw_closing.
+  easy.
+Qed.
+
+Lemma raw_closing_associative r1 r2 r3 :
+  normalized_pushes r3 ->
+  compose_raw_closing r1 (compose_raw_closing r2 r3)
+  = compose_raw_closing (compose_raw_closing r1 r2) r3.
+Proof.
+  generalize dependent r2.
+  generalize dependent r3.
+  induction r1; cbn; intros r3 r2 Hnorm; try easy.
+  rewrite compose_normalized_pushes_cons by easy; cbn.
+  rewrite !rhs_push_transpose_push_raw_closing,
+    !rhs_raw_closing_transpose_push_raw_closing.
+  rewrite transpose_push_compose_raw_closing_raw_closing
+    by easy.
+  rewrite IHr1
+    by (apply transpose_push_raw_closing_raw_closing_normalized;
+        easy).
+  rewrite transpose_push_compose_raw_closing_push.
+  easy.
+Qed.
+
+Lemma closing_associative r1 r2 r3 :
+  compose_closing r1 (compose_closing r2 r3)
+  = compose_closing (compose_closing r1 r2) r3.
+Proof.
+  destruct r1, r2, r3.
+  apply lift_closing_eq; cbn.
+  apply raw_closing_associative; easy.
+Qed.
